improve

srv.v
@@ -45,6 +45,7 @@ Global Opaque doOp install loop flat.
 
 Definition srvR := prodR fracR (dec_agreeR val).
 Definition tokR := evmapR loc (gname * gname * gname * gname).
+Definition srvmR := evmapR loc val.
 Class srvG Σ := SrvG {
   srv_G :> inG Σ srvR;
   tok_G :> inG Σ (authR tokR);
@@ -68,7 +69,7 @@ Section proof.
     (∃ (p : loc) (q: Qp), v = #p ★ own γm (◯ ({[ p := (q, DecAgree (γx, γ1, γ3, γ4)) ]} : tokR)) ★
      ((∃ (y: val), p ↦{1/2} InjRV y ★ own γ1 (Excl ()) ★ own γ3 (Excl ())) ∨
       (∃ (x: val), p ↦{1/2} InjLV x ★ own γx ((1/2)%Qp, DecAgree x) ★ own γ1 (Excl ()) ★ own γ4 (Excl ())) ∨
-      (∃ (x: val), p ↦{1/2} InjLV x ★ own γx ((1/4)%Qp, DecAgree x) ★ own γ2 (Excl ()) ★ own γ4 (Excl ())) ∨
+      (∃ (x: val), p ↦{1/2} InjLV x ★ own γx ((1/2/2)%Qp, DecAgree x) ★ own γ2 (Excl ()) ★ own γ4 (Excl ())) ∨
       (∃ (x y: val), p ↦{1/2} InjRV y ★ own γx ((1/2)%Qp, DecAgree x) ★ ■ Q x y ★ own γ1 (Excl ()) ★ own γ4 (Excl ()))))%I.
 
   Definition p_inv_R γm γ2 Q v : iProp Σ :=
@@ -84,42 +85,43 @@ Section proof.
         (p: loc) (γ γm γx γ1 γ2 γ3 γ4: gname)
         (s: loc) (x: val) :
     heapN ⊥ N →
-    heap_ctx ★ inv N (srv_stack_inv γ γm γ2 s Q) ★ own γx ((1/2)%Qp, DecAgree x) ★
+    heap_ctx ★ inv N (srv_stack_inv γ γm γ2 s Q ★ srv_m_inv γm) ★ own γx ((1/2)%Qp, DecAgree x) ★
     own γm (◯ ({[ p := ((1 / 2)%Qp, DecAgree (γx, γ1, γ3, γ4)) ]})) ★
-    p ↦{1/2} InjLV x ★ own γ1 (Excl ()) ★ own γ4 (Excl ()) ★ (True -★ Φ #())
+    p ↦{1/2} InjLV x ★ own γ1 (Excl ()) ★ own γ4 (Excl ()) ★ ((∃ (hd : loc) (q : Qp), ev γ hd q #p) -★ Φ #())
     ⊢ WP push #s #p {{ Φ }}.
   Proof.
     iIntros (HN) "(#Hh & #? & Hx & Hpm & Hp & Ho1 & Ho2 & HΦ)".
     rewrite /srv_stack_inv.
-    iDestruct (push_spec N (p_inv_R γm γ2 Q) with "[-HΦ]") as "Hpush"=>//.
+    iDestruct (push_spec N (p_inv_R γm γ2 Q) (fun v => (∃ (hd : loc) (q : Qp), ev γ hd q #p) ★ v = #())%I
+               with "[-HΦ]") as "Hpush"=>//.
     - iFrame "Hh". iSplitL "Hx Hp Hpm Ho1 Ho2"; last eauto.
       iExists γx, γ1, γ3, γ4. iExists p, (1/2)%Qp. iSplit=>//. iFrame "Hpm".
       iRight. iLeft.
       iExists x. iFrame.
     - iApply wp_wand_r.
       iSplitL "Hpush"; first done.
-      iIntros (?). iIntros "%".
-      inversion H. by iApply "HΦ".
+      iIntros (?) "[? %]". subst.
+      by iApply "HΦ".
   Qed.
 
   Lemma install_spec
         (Φ: val → iProp Σ) (Q: val → val → Prop)
         (x: val) (γ2 γm γ: gname) (s: loc):
     heapN ⊥ N →
-    heap_ctx ★ inv N (srv_stack_inv γ γm γ2 s Q) ★ inv N (srv_m_inv γm) ★ 
+    heap_ctx ★ inv N (srv_stack_inv γ γm γ2 s Q ★ srv_m_inv γm) ★ 
     (∀ (p: loc) (γx γ1 γ2 γ3 γ4: gname),
        own γ3 (Excl ()) -★ own γm (◯ {[ p := ((1 / 2)%Qp, DecAgree (γx, γ1, γ3, γ4)) ]}) -★
-       own γx ((1/2)%Qp, DecAgree x) -★ Φ #p)
+       own γx ((1/2)%Qp, DecAgree x) -★ (∃ (hd : loc) (q : Qp), ev γ hd q #p) -★ Φ #p)
     ⊢ WP install x #s {{ Φ }}.
   Proof.
-    iIntros (HN) "(#Hh & #? & #? & HΦ)".
+    iIntros (HN) "(#Hh & #? & HΦ)".
     wp_seq. wp_let. wp_alloc p as "Hl".
     iApply pvs_wp.
     iVs (own_alloc (Excl ())) as (γ1) "Ho1"; first done.
     iVs (own_alloc (Excl ())) as (γ3) "Ho3"; first done.
     iVs (own_alloc (Excl ())) as (γ4) "Ho4"; first done.
     iVs (own_alloc (1%Qp, DecAgree x)) as (γx) "Hx"; first done.
-    iInv N as ">Hm" "Hclose".
+    iInv N as ">[Hrs Hm]" "Hclose".
     iDestruct "Hm" as (m) "[Hm HRm]".
     destruct (m !! p) eqn:Heqn.
     - (* old name *)
@@ -131,8 +133,8 @@ Section proof.
       { iDestruct (own_update with "Hm") as "?"; last by iAssumption.
         apply auth_update_no_frag. apply alloc_unit_singleton_local_update=>//. }
       iDestruct "Hl" as "[Hl1 Hl2]".
-      iVs ("Hclose" with "[HRm Hm1 Hl1]").
-      + iNext. rewrite /srv_m_inv. iExists ({[p := (1%Qp, DecAgree (γx, γ1, γ3, γ4))]} ⋅ m).
+      iVs ("Hclose" with "[HRm Hm1 Hl1 Hrs]").
+      + iNext. iFrame. rewrite /srv_m_inv.  iExists ({[p := (1%Qp, DecAgree (γx, γ1, γ3, γ4))]} ⋅ m).
         iFrame.
         replace ({[p := (1%Qp, DecAgree (γx, γ1, γ3, γ4))]} ⋅ m) with
                 (<[p := (1%Qp, DecAgree (γx, γ1, γ3, γ4))]> m); last by apply insert_singleton_op.
@@ -147,9 +149,10 @@ Section proof.
         iDestruct (own_update with "Hx") as "==>[Hx1 Hx2]"; first by apply pair_l_frac_op_1'.
         iVsIntro. wp_let. wp_bind ((push _) _).
         iApply install_push_spec=>//.
-        iFrame "#". iFrame "Hx1 Hfrag1 Hl2 Ho1 Ho4". iIntros "_". wp_seq. iVsIntro.
-        iSpecialize ("HΦ" $! p γx γ1 γ2 γ3 γ4 with "[-Hx2 Hfrag2]")=>//.
-        iApply ("HΦ" with "Hfrag2 Hx2"). 
+        iFrame "#". iFrame "Hx1 Hfrag1 Hl2 Ho1 Ho4".
+        iIntros "Hev". wp_seq. iVsIntro.
+        iSpecialize ("HΦ" $! p γx γ1 γ2 γ3 γ4 with "[-Hx2 Hfrag2 Hev]")=>//.
+        by iApply ("HΦ" with "Hfrag2 Hx2").
   Qed.
 
   Lemma access x xs m Q (γ γm γ2: gname):
@@ -160,7 +163,7 @@ Section proof.
     is_list' γ hd xs
     ⊢ ∃ hd', (([★ map] _↦v ∈ delete hd' m, ∃ v' : val,
                                            v = (1%Qp, DecAgree v') ★ p_inv_R γm γ2 Q v') ★
-         ∃ v, v = (1%Qp, DecAgree x) ★ p_inv_R γm γ2 Q x) ★ own γ (● m).
+         ∃ v, v = (1%Qp, DecAgree x) ★ p_inv_R γm γ2 Q x ★ m !! hd' = Some v) ★ own γ (● m).
   Proof.
     induction xs as [|x' xs' IHxs'].
     - iIntros (? _ Habsurd). inversion Habsurd.
@@ -193,131 +196,295 @@ Section proof.
         iApply IHxs'=>//.
         iFrame "#". iFrame.
   Qed.
-    
+
+  Lemma map_agree_none' {A: cmraT} m m' (hd: loc) (q: A) (x: gname * gname * gname * gname):
+    m !! hd = None → m = {[hd := (q, DecAgree x)]} ⋅ m' → False.
+  Proof.
+    intros H1 H2. subst. rewrite lookup_op lookup_singleton in H1.
+    destruct (m' !! hd)=>//.
+  Qed.
+
+  Lemma m_frag_agree' γm p q1 q2 (γs1 γs2: gname * gname * gname * gname):
+    own γm (◯ {[p := (q1, DecAgree γs1)]}) ★
+    own γm (◯ {[p := (q2, DecAgree γs2)]})
+    ⊢ |=r=> own γm (◯ {[p := ((q1 + q2)%Qp, DecAgree γs1)]}) ★ (γs1 = γs2).
+  Proof.
+    iIntros "[Ho Ho']".
+    destruct (decide (γs1 = γs2)) as [->|Hneq].
+    - iSplitL=>//.
+      iCombine "Ho" "Ho'" as "Ho".
+      iDestruct (own_update with "Ho") as "?"; last by iAssumption.
+      rewrite <-(@auth_frag_op tokR {[p := (q1, DecAgree γs2)]} {[p := (q2, DecAgree γs2)]}).
+      by rewrite op_singleton pair_op frac_op' dec_agree_idemp.
+    - iCombine "Ho" "Ho'" as "Ho".
+      iDestruct (own_valid with "Ho") as %Hvalid.
+      exfalso. rewrite <-(@auth_frag_op tokR) in Hvalid.
+      rewrite op_singleton in Hvalid.
+      apply auth_valid_discrete in Hvalid. simpl in Hvalid.
+      apply singleton_valid in Hvalid.
+      destruct Hvalid as [_ Hvalid].
+      apply dec_agree_op_inv in Hvalid. inversion Hvalid. subst. auto.
+  Qed.
+
+    Lemma m_frag_agree γm q1 q2 (γs1 γs2: val):
+    own γm (q1, DecAgree γs1) ★ own γm (q2, DecAgree γs2)
+    ⊢ |=r=> own γm ((q1 + q2)%Qp, DecAgree γs1) ★ (γs1 = γs2).
+  Proof.
+    iIntros "[Ho Ho']".
+    destruct (decide (γs1 = γs2)) as [->|Hneq].
+    - iSplitL=>//.
+      iCombine "Ho" "Ho'" as "Ho".
+      iDestruct (own_update with "Ho") as "?"; last by iAssumption.
+      by rewrite pair_op frac_op' dec_agree_idemp.
+    - iCombine "Ho" "Ho'" as "Ho".
+      iDestruct (own_valid with "Ho") as %Hvalid.
+      exfalso. destruct Hvalid as [_ Hvalid].
+      simpl in Hvalid. apply dec_agree_op_inv in Hvalid. inversion Hvalid. subst. auto.
+  Qed.
+
+  Lemma in_m (m: srvmR) k q q' (a b: val) γ:
+    m !! k = Some (q, DecAgree a) →
+    own γ (● m) ★ own γ (◯ {[ k := (q', DecAgree b)]})
+    ⊢ own γ (● m) ★ own γ (◯ {[ k := (q', DecAgree a)]}) ★ a = b.
+  Proof.
+    iIntros (H) "[HFull HFrag]".
+    destruct (decide (a = b)).
+    - subst. by iFrame.
+    - iCombine "HFull" "HFrag" as "Hauth".
+      iDestruct (own_valid γ (● m ⋅ ◯ {[k := (q', DecAgree b)]}) with "[Hauth]") as %Hvalid=>//. 
+      exfalso. apply auth_valid_discrete_2 in Hvalid as [[af Compose%leibniz_equiv_iff] Valid].
+      eapply (map_agree m af)=>//. rewrite Compose in H. done.
+  Qed.
+
   Lemma loop_iter_list_spec Φ (f: val) (s hd: loc) Q (γ γm γ2: gname) xs:
     heapN ⊥ N → (∀ x:val, True ⊢ WP f x {{ v, ■ Q x v }}) →
-    heap_ctx ★ inv N (srv_stack_inv γ γm γ2 s Q) ★ own γ2 (Excl ()) ★
+    heap_ctx ★ inv N (srv_stack_inv γ γm γ2 s Q ★ srv_m_inv γm) ★ own γ2 (Excl ()) ★
     is_list' γ hd xs ★ (own γ2 (Excl ()) -★ Φ #())
     ⊢ WP iter' #hd (doOp f) {{ Φ }}.
   Proof.
-    iIntros (HN Hf) "(#Hh & #? & Ho2 & Hlist' & HΦ)".
+    iIntros (HN Hf) "(#? & #? & Ho2 & Hlist' & HΦ)".
     iApply pvs_wp.
     iDestruct (dup_is_list' with "[Hlist']") as "==>[Hl1 Hl2]"; first by iFrame.
     iDestruct (dup_is_list' with "[Hl2]") as "==>[Hl2 Hl3]"; first by iFrame.
-    iDestruct (iter'_spec _ (p_inv_R γm γ2 Q) _ γ s (is_list' γ hd xs ★ own γ2 (Excl ()))%I xs hd
+    iVsIntro.
+    iDestruct (iter'_spec _ (p_inv_R γm γ2 Q) (fun v => v = #() ★ own γ2 (Excl ()))%I γ s (is_list' γ hd xs ★ own γ2 (Excl ()))%I (srv_m_inv γm) xs hd
                           (doOp f) (doOp f)
-              with "[-Hl1]") as "Hiter'"=>//.
-    - rewrite /f_spec.
+              with "[-Hl1 HΦ]") as "Hiter'"=>//.
+    - rewrite /f_spec. 
       iIntros (Φ' p _ Hin) "(#Hh & #? & (Hls & Ho2) & HΦ')".
-      wp_let. wp_bind (! _)%E. iInv N as (xs') ">Hs" "Hclose".
-      iDestruct "Hs" as (hd') "[Hhd [Hxs HRs]]".
+      wp_let. wp_bind (! _)%E. iInv N as ">[Hs Hm]" "Hclose".
+      iDestruct "Hs" as (xs' hd') "[Hhd [Hxs HRs]]".
       iDestruct (dup_is_list' with "[Hls]") as "==>[Hls1 Hls2]"; first by iFrame.
       iDestruct "HRs" as (m) "[Hom HRs]".
-      iDestruct (access with "[Hom HRs Hls1]") as "[Hop Hom]"=>//.
-      { iFrame "#". iFrame. }
-      iDestruct "Hop" as (p') "[Hos Ho]".
-      iDestruct "Ho" as (v) "[% Hv']". subst.
-      iDestruct "Hv'" as (γx γ1 γ3 γ4) "H".
-      iDestruct "H" as (p'' q'') "[% [Ho [Hp | [Hp | [Hp | Hp]]]]]"; subst.
-      + iDestruct "Hp" as (y) "(Hp'' & Ho1 & Ho3)".
+      iDestruct (access with "[Hom HRs Hls1]") as (hd'') "[[Hops Hop2] Hom']"=>//; first by iFrame.
+      iDestruct "Hop2" as ([q x]) "(% & H & %)".
+      iDestruct "H" as (γx γ1 γ3 γ4 p'' q'') "[% [Hop [Hp | [Hp | [Hp | Hp]]]]]"; subst.
+      + iDestruct "Hp" as (x') "(Hp & Ho1 & Ho3)".
         wp_load. iVs ("Hclose" with "[-HΦ' Ho2 Hls2]").
-        { iNext. iExists xs', hd'. iFrame.
-          iAssert (p_inv_R γm γ2 Q #p'') with "[-Hom Hos]" as "HIp''".
-          { iExists γx, γ1, γ3, γ4, p'', q''.
-            iSplitR; first done. iFrame.
-            iLeft. iExists y. by iFrame. }
-          iExists m. iFrame. admit. }
+        { iNext. iFrame. iExists xs', hd'.
+          iFrame "Hhd Hxs". iExists m.
+          iFrame "Hom'". iDestruct (merge_mapv m with "[Hop Hops Hp Ho1 Ho3]") as "?"=>//.
+          iFrame. iExists #p''. iSplitR; first auto. iExists γx, γ1, γ3, γ4, p'', q''.
+          iSplitR; auto. iFrame. iLeft. iExists x'. iFrame. }
         iVsIntro. wp_match. iApply "HΦ'". iFrame.
-      + (* major part of proof ... *)
-        admit.
-      + iExFalso. admit.
-      + (* same as the first one *)
-        admit.
+      + iDestruct "Hp" as (x') "(Hp & Hx & Ho1 & Ho4)".
+        wp_load.
+        iAssert (|=r=> own γm (◯ {[p'' := ((q''/2)%Qp, DecAgree (γx, γ1, γ3, γ4))]} ⋅
+                               ◯ {[p'' := ((q''/2)%Qp, DecAgree (γx, γ1, γ3, γ4))]}))%I
+                with "[Hop]" as "==>[Hop1 Hop2]".
+        { iDestruct (own_update with "Hop") as "?"; last by iAssumption.
+          rewrite <-auth_frag_op.
+          by rewrite op_singleton pair_op dec_agree_idemp frac_op' Qp_div_2.
+        }
+        iAssert (|=r=> own γx (((1 / 2 / 2)%Qp, DecAgree x') ⋅ ((1 / 2/ 2)%Qp, DecAgree x')))%I with "[Hx]" as "==>[Hx1 Hx2]".
+        { iDestruct (own_update with "Hx") as "?"; last by iAssumption.
+          rewrite -{1}(Qp_div_2 (1/2)%Qp).
+          by apply pair_l_frac_op'. }
+        iVs ("Hclose" with "[-Hls2 Ho1 Hx2 Hop2 HΦ']").
+        { iNext. iFrame. iExists xs', hd'.
+          iFrame "Hhd Hxs". iExists m.
+          iFrame "Hom'". iDestruct (merge_mapv m with "[Hop1 Hops Hp Hx1 Ho2 Ho4]") as "?"=>//.
+          simpl. iFrame. iExists #p''.  iSplitR; auto.
+          iExists γx, γ1, γ3, γ4, p'', (q''/2)%Qp. iSplitR; auto.
+          iFrame. iRight. iRight. iLeft. iExists x'. iFrame. }
+        iVsIntro. wp_match.
+        wp_bind (f _). iApply wp_wand_r. iSplitR; first iApply Hf.
+        iIntros (v) "%".
+        wp_value. iVsIntro. iInv N as ">[Hs Hm]" "Hclose".
+        iDestruct "Hs" as (xs'' hd''') "[Hhd [Hxs HRs]]".
+        iDestruct "HRs" as (m') "[Hom HRs]".
+        iDestruct (dup_is_list' with "[Hls2]") as "==>[Hls2 Hls3]"; first by iFrame.
+        iDestruct (access with "[Hom HRs Hls2]") as (hd'''') "[[Hops Hop3] Hom']"=>//; first by iFrame.
+        iDestruct "Hop3" as ([q''' x''']) "(% & H & %)".
+        iDestruct "H" as (γx' γ1' γ3' γ4' p'''' q'''') "[% [Hop Hps]]".
+        inversion H4.
+        destruct (decide (γ1 = γ1' ∧ γx = γx' ∧ γ3 = γ3' ∧ γ4 = γ4')) as [[? [? [? ?]]]|Hneq].
+        { 
+          subst.
+          iDestruct "Hps" as "[Hp | [Hp | [Hp | Hp]]]".
+          * iDestruct "Hp" as (x5) "(Hp & Ho1' & Ho3)". iExFalso.
+            iCombine "Ho1" "Ho1'" as "Ho1".
+            by iDestruct (own_valid with "Ho1") as "%".
+          * iDestruct "Hp" as (x5) "(Hp & Hx & Ho1' & Ho3)".
+            iExFalso. iCombine "Ho1" "Ho1'" as "Ho1".
+            by iDestruct (own_valid with "Ho1") as "%".
+          * iDestruct "Hp" as (x5) "(Hp & Hx & Ho2 & Ho4)".
+            iDestruct "Hm" as (m2) "[Hom2 HRm]".
+            destruct (m2 !! p'''') eqn:Heqn.
+            { 
+              iDestruct (split_mapk m2 with "[HRm]") as "[HRk HRm]"=>//.
+              iDestruct "HRk" as (?) "HRk".
+              iDestruct (heap_mapsto_op_1 with "[HRk Hp]") as "[% Hp]"; first by iFrame.
+              rewrite Qp_div_2. wp_store.
+              (* now close the invariant *)
+              iDestruct (m_frag_agree with "[Hx Hx2]") as "==>[Hx %]"; first iFrame.
+              subst.
+              rewrite Qp_div_2.
+              iVs ("Hclose" with "[-HΦ' Ho2 Hls3]").
+              { iNext.
+                iDestruct "Hp" as "[Hp1 Hp2]".
+                iAssert (srv_m_inv γm) with "[Hp1 HRm Hom2]" as "HRm".
+                { iExists m2. iFrame. iApply (merge_mapk m2)=>//.
+                  iFrame. eauto. }
+                iFrame. iExists xs''. iFrame. iExists hd'''. iFrame.
+                iExists m'. iFrame.
+                iDestruct (merge_mapv m' with "[-]") as "?"=>//.
+                { simpl. iFrame. rewrite H2. iExists #p''''.
+                  iSplitR; first auto. iExists γx', γ1', γ3', γ4'.
+                  rewrite /p_inv. iExists p'''', q''''.
+                  iSplitR; first auto. iFrame. iRight. iRight.
+                  iRight. iExists x5, v. iFrame. done. }
+              }
+              iApply "HΦ'". iFrame. 
+            }
+            { iExFalso.
+              iCombine "Hom2" "Hop2" as "Hauth".
+              iDestruct (own_valid γm (● m2
+                ⋅ ◯ {[p''''
+                    := ((q'' / 2)%Qp, DecAgree (γx', γ1', γ3', γ4'))]}) with "[Hauth]") as %Hvalid=>//.
+              iPureIntro.
+              apply auth_valid_discrete_2 in Hvalid as [[af Compose%leibniz_equiv_iff] Valid].
+              eapply map_agree_none'=>//. }
+          * iDestruct "Hp" as (? ?) "(_ & _ & _ & Ho1' & _)".
+            iExFalso. iCombine "Ho1" "Ho1'" as "Ho1".
+            by iDestruct (own_valid with "Ho1") as "%". }
+        { iDestruct (m_frag_agree' with "[Hop Hop2]") as "==>[Hop %]"; first iFrame.
+           inversion H5. subst. exfalso. apply Hneq. auto. }
+      + iDestruct "Hp" as (y) "(Hp & Hx & Ho2' & Ho4)".
+        iExFalso. iCombine "Ho2" "Ho2'" as "Ho2".
+        by iDestruct (own_valid with "Ho2") as "%".
+      + iDestruct "Hp" as (x' y) "(Hp & Ho1 & Ho4)".
+        wp_load. iVs ("Hclose" with "[-HΦ' Ho2 Hls2]").
+        { iNext. iFrame. iExists xs', hd'.
+          iFrame "Hhd Hxs". iExists m.
+          iFrame "Hom'". iDestruct (merge_mapv m with "[Hop Hops Hp Ho1 Ho4]") as "?"=>//.
+          iFrame. iExists #p''. iSplitR; first auto. iExists γx, γ1, γ3, γ4, p'', q''.
+          iSplitR; auto. iFrame. iRight. iRight. iRight. iExists x', y. iFrame. }
+        iVsIntro. wp_match. iApply "HΦ'". iFrame.
     - apply to_of_val.
-    - iFrame "#". iFrame "Hl2 Hl3 Ho2".
-      iIntros "[_ H]". by iApply "HΦ".
-    - done.
-  Admitted.
-
+    - rewrite /srv_stack_inv. iFrame "#". iFrame. iIntros "[_ Ho2]". eauto.
+    - iApply wp_wand_r. iSplitL "Hiter'"; first done.
+      iIntros (?) "[% Ho2]". subst. by iApply "HΦ".
+  Qed.
+      
   Lemma loop_spec Φ (p s: loc) (lk: val) (f: val)
         Q (γ2 γm γ γlk: gname) (γx γ1 γ3 γ4: gname):
     heapN ⊥ N → (∀ x:val, True ⊢ WP f x {{ v, ■ Q x v }}) →
-    heap_ctx ★ inv N (srv_stack_inv γ γm γ2 s Q) ★ is_lock N γlk lk (own γ2 (Excl ())) ★
+    heap_ctx ★ inv N (srv_stack_inv γ γm γ2 s Q ★ srv_m_inv γm) ★ is_lock N γlk lk (own γ2 (Excl ())) ★
     own γ3 (Excl ()) ★ (∃ q: Qp, own γm (◯ {[ p := (q, DecAgree (γx, γ1, γ3, γ4)) ]})) ★
-    (∀ x y,  own γx ((1 / 2)%Qp, DecAgree x) -★ ■ Q x y -★  Φ y)
+    (∃ hd q, ev γ hd q #p) ★ (∀ x y,  own γx ((1 / 2)%Qp, DecAgree x) -★ ■ Q x y -★ Φ y)
     ⊢ WP loop f #p #s lk {{ Φ }}.
   Proof.
-    iIntros (HN Hf) "(#Hh & #? & #? & Ho3 & Hγs & HΦ)".
+    iIntros (HN Hf) "(#Hh & #? & #? & Ho3 & Hγs & Hev & HΦ)".
     iLöb as "IH". wp_rec. repeat wp_let.
     iDestruct "Hγs" as (q) "Hγs".
-    wp_bind (! _)%E. iInv N as ">Hinv" "Hclose".
+    wp_bind (! _)%E. iInv N as ">[Hinv ?]" "Hclose". 
     iDestruct "Hinv" as (xs hd) "[Hs [Hxs HRs]]".
     iDestruct "HRs" as (m) "[Hom HRs]".
-    destruct (decide (m !! p = None)).
-    (* There is also problem regarding destruct the cases of lookup ... *)
-    - admit. (* impossible -- because of the fragment *)
-    - iAssert (([★ map] _↦v ∈ delete p m, ∃ v' : val, v = (1%Qp, DecAgree v') ★ p_inv_R γm γ2 Q v') ★
-               (∃ v, v = (1%Qp, DecAgree #p) ★ p_inv_R γm γ2 Q #p))%I
-              with "[HRs]" as "[HRs Hp]".
-      { admit. (* lookup case analysis problem *)
-        (* iDestruct (big_sepM_delete with "[HRs]") as "H". *) }
+    iDestruct "Hev" as (hdp ?) "Hev".
+    rewrite /ev. destruct (m !! hdp) eqn:Heqn.
+    - iDestruct (split_mapv m with "[HRs]") as "[Hp Hrs]"=>//.
       iDestruct "Hp" as (?) "[% Hpr]"; subst.
       iDestruct "Hpr" as (γx' γ1' γ3' γ4' p' q') "(% & Hp' & Hp)".
-      inversion H. subst.
-      destruct (decide (γ1 = γ1' ∧ γx = γx' ∧ γ3 = γ3' ∧ γ4 = γ4')) as [[? [? [? ?]]]|Hneq].
-      + subst. 
-        iDestruct "Hp" as "[Hp | [Hp | [ Hp | Hp]]]".
-        * (* trivial *) admit.
-        * iDestruct "Hp" as (x) "(Hp & Hx & Ho1 & Ho4)".
-          wp_load.
-          iVs ("Hclose" with "[-Hp' Ho3 HΦ]").
-          { iNext. iExists xs, hd. iFrame. iExists m. iFrame. (* merge *) admit. }
-          iVsIntro. wp_match. (* we should close it as it is in this case *)
-          (* now, just reason like a server *)
-          wp_bind (try_acquire _). iApply try_acquire_spec.
-          iFrame "#". iSplit.
-          { (* acquired the lock *)
-            iIntros "Hlocked Ho2".
-            wp_if. wp_bind ((iter' _) _). wp_bind (! _)%E.
-            iInv N as ">H" "Hclose".
-            iDestruct "H" as (xs' hd') "[Hs [Hxs HRs]]".
-            wp_load. iDestruct (dup_is_list' with "[Hxs]") as "==>[Hxs1 Hxs2]"; first by iFrame.
-            iVs ("Hclose" with "[Hs Hxs1 HRs]").
-            { iNext. iExists xs', hd'. by iFrame. }
-            iVsIntro. iApply loop_iter_list_spec=>//.
-            iFrame "#". iFrame. iIntros "Ho2".
-            wp_seq. wp_bind (release _). iApply release_spec.
-            iFrame "~ Hlocked Ho2". wp_seq.
-            iAssert ((∃ q0 : Qp,
-                        own γm (◯ {[p' := (q0, DecAgree (γx', γ1', γ3', γ4'))]})))%I with "[Hp']" as "Hp'".
+      subst. iDestruct (in_m with "[Hom Hev]") as "(Hom & Hev & %)"=>//; first iFrame.
+      inversion H0. subst.
+      iDestruct (m_frag_agree' with "[Hγs Hp']") as "==>[Hγs %]"; first iFrame.
+      inversion H1. subst.
+      iDestruct "Hp" as "[Hp | [Hp | [ Hp | Hp]]]".
+      + (* trivial *) admit.
+      + iDestruct "Hp" as (x) "(Hp & Hx & Ho1 & Ho4)".
+        wp_load.
+        iVs ("Hclose" with "[-Hγs Ho3 HΦ Hev]"). (* Hev here should be a duplicated one *)
+        { iNext. iFrame. iExists xs, hd. iFrame. iExists m. iFrame. (* merge *) admit. }
+        iVsIntro. wp_match. (* we should close it as it is in this case *)
+        (* now, just reason like a server *)
+        wp_bind (try_acquire _). iApply try_acquire_spec.
+        iFrame "#". iSplit.
+        { (* acquired the lock *)
+          iIntros "Hlocked Ho2".
+          wp_if. wp_bind ((iter' _) _). wp_bind (! _)%E.
+          iInv N as ">[H Hm]" "Hclose".
+          iDestruct "H" as (xs' hd') "[Hs [Hxs HRs]]".
+          wp_load. iDestruct (dup_is_list' with "[Hxs]") as "==>[Hxs1 Hxs2]"; first by iFrame.
+          iVs ("Hclose" with "[Hs Hxs1 HRs Hm]").
+          { iNext. iFrame. iExists xs', hd'. by iFrame. }
+          iVsIntro. iApply loop_iter_list_spec=>//.
+          iFrame "#". iFrame. iIntros "Ho2".
+          wp_seq. wp_bind (release _). iApply release_spec.
+          iFrame "~ Hlocked Ho2". wp_seq.
+          iAssert ((∃ q0 : Qp,
+                      own γm (◯ {[p := (q0, DecAgree (γx, γ1, γ3, γ4))]})))%I with "[Hγs]" as "Hγs".
+          { eauto. }
+          iAssert (∃ (hd0 : loc) (q0 : Qp), own γ (◯ {[hd0 := (q0, DecAgree #p)]}))%I with "[Hev]" as "Hev".
+          { eauto. }
+          by iApply ("IH" with "Ho3 Hγs Hev"). }
+        {  wp_if.
+           iAssert ((∃ q0 : Qp,
+                        own γm (◯ {[p := (q0, DecAgree (γx, γ1, γ3, γ4))]})))%I with "[Hγs]" as "Hp'".
             { eauto. }
-            by iApply ("IH" with "Ho3 Hp'"). }
-          {  wp_if.
-            iAssert ((∃ q0 : Qp,
-                        own γm (◯ {[p' := (q0, DecAgree (γx', γ1', γ3', γ4'))]})))%I with "[Hp']" as "Hp'".
-            { eauto. }
-            iApply ("IH" with "Ho3 Hp'")=>//. }
-        * iDestruct "Hp" as (x) "(Hp & Hx & Ho1 & Ho4)".
+          iAssert (∃ (hd0 : loc) (q0 : Qp), own γ (◯ {[hd0 := (q0, DecAgree #p)]}))%I with "[Hev]" as "Hev".
+          { eauto. }
+            iApply ("IH" with "Ho3 Hp' Hev")=>//. }
+      + iDestruct "Hp" as (x) "(Hp & Hx & Ho2 & Ho4)".
+        wp_load.
+        iVs ("Hclose" with "[-Hγs Ho3 HΦ Hev]").
+        { iNext. iFrame. iExists xs, hd. iFrame. iExists m. iFrame. (* merge *) admit. }
+        iVsIntro. wp_match.
+        (* now, just reason like a server *)
+        wp_bind (try_acquire _). iApply try_acquire_spec.
+        iFrame "#". iSplit.
+        { (* acquired the lock *)
+          iIntros "Hlocked Ho2".
+          wp_if. wp_bind ((iter' _) _). wp_bind (! _)%E.
+          iInv N as ">[H Hm]" "Hclose".
+          iDestruct "H" as (xs' hd') "[Hs [Hxs HRs]]".
+          wp_load. iDestruct (dup_is_list' with "[Hxs]") as "==>[Hxs1 Hxs2]"; first by iFrame.
+          iVs ("Hclose" with "[Hs Hxs1 HRs Hm]").
+          { iNext. iFrame. iExists xs', hd'. by iFrame. }
+          iVsIntro. iApply loop_iter_list_spec=>//.
+          iFrame "#". iFrame. iIntros "Ho2".
+          wp_seq. wp_bind (release _). iApply release_spec.
+          iFrame "~ Hlocked Ho2". wp_seq.
+          iAssert ((∃ q0 : Qp,
+                      own γm (◯ {[p := (q0, DecAgree (γx, γ1, γ3, γ4))]})))%I with "[Hγs]" as "Hγs".
+          { eauto. }
+          iAssert (∃ (hd0 : loc) (q0 : Qp), own γ (◯ {[hd0 := (q0, DecAgree #p)]}))%I with "[Hev]" as "Hev".
+          { eauto. }
+            by iApply ("IH" with "Ho3 Hγs Hev"). }
+        {  wp_if.
+           iAssert ((∃ q0 : Qp,
+                       own γm (◯ {[p := (q0, DecAgree (γx, γ1, γ3, γ4))]})))%I with "[Hγs]" as "Hp'".
+           { eauto. }
+           iAssert (∃ (hd0 : loc) (q0 : Qp), own γ (◯ {[hd0 := (q0, DecAgree #p)]}))%I with "[Hev]" as "Hev".
+          { eauto. }
+            iApply ("IH" with "Ho3 Hp' Hev")=>//. }
+            (* the #2 and #3 processing are identical *)
+      + iDestruct "Hp" as (x y) "(Hp & Hox & % & Ho1 & Ho4)".
           wp_load.
-          iVs ("Hclose" with "[-Hp' Ho3 HΦ]").
-          { iNext. iExists xs, hd. iFrame. iExists m. iFrame. (* merge *) admit. }
-          iVsIntro. wp_match.
-          wp_bind (try_acquire _). iApply try_acquire_spec.
-          iFrame "#". iSplit.
-          { (* impossible *) admit. }
-          { wp_if.
-            iAssert ((∃ q0 : Qp,
-                        own γm (◯ {[p' := (q0, DecAgree (γx', γ1', γ3', γ4'))]})))%I with "[Hp']" as "Hp'".
-            { eauto. }
-            iApply ("IH" with "Ho3 Hp'")=>//. }
-        * iDestruct "Hp" as (x y) "(Hp & Hox & % & Ho1 & Ho4)".
-          wp_load.
-          iVs ("Hclose" with "[-Hp' Ho3 HΦ Hox]").
-          { iNext. iExists xs, hd. iFrame. iExists m. iFrame. (* merge *) admit. }
+          iVs ("Hclose" with "[-Hγs Ho3 HΦ Hox]").
+          { iNext. iFrame. iExists xs, hd. iFrame. iExists m. iFrame. (* merge *) admit. }
           iVsIntro. wp_match. by iApply ("HΦ" with "Hox").
-      + iCombine "Hγs" "Hp'" as "Hγs".
-        iExFalso.
-        admit.
+    - iExFalso. admit. (* this is the second hardest part *)
   Admitted.
 
   Lemma flat_spec (f: val) Q:
@@ -328,20 +495,20 @@ Section proof.
     iVs (own_alloc (Excl ())) as (γ2) "Ho2"; first done.
     iVs (own_alloc (● (∅: tokR) ⋅ ◯ ∅)) as (γm) "[Hm _]".
     { by rewrite -auth_both_op. }
-    iVs (inv_alloc N _ (srv_m_inv γm)%I with "[Hm]") as "#Hm"; first eauto.
-    { iNext. rewrite /srv_m_inv. iExists ∅. iFrame. (* XXX: iApply big_sepM_empty. *)
+    iAssert (srv_m_inv γm) with "[Hm]" as "Hm"; first eauto.
+    { rewrite /srv_m_inv. iExists ∅. iFrame. (* XXX: iApply big_sepM_empty. *)
       by rewrite /uPred_big_sepM map_to_list_empty. }
     wp_seq. wp_bind (newlock _).
     iApply newlock_spec=>//.
     iFrame "Hh Ho2". iIntros (lk γlk) "#Hlk".
     wp_let. wp_bind (new_stack _).
     iApply (new_stack_spec' _ (p_inv_R γm γ2 Q))=>//.
-    iFrame "Hh". iIntros (γ s) "#Hss".
+    iFrame "Hh Hm". iIntros (γ s) "#Hss".
     wp_let. iVsIntro. iAlways.
     iIntros (x). wp_let.
     wp_bind ((install _) _).
     iApply install_spec=>//.
-    iFrame "Hh Hss Hm". iIntros (p γx γ1 _ γ3 γ4) "Hp3 Hpx Hx".
+    iFrame "Hh Hss". iIntros (p γx γ1 _ γ3 γ4) "Hp3 Hpx Hx Hev".
     wp_let. iApply loop_spec=>//.
     iFrame "Hh Hss Hlk". iFrame.
     iSplitL "Hpx"; first eauto.
